add chunk view functions

crypto_examples/ntt.dfy
@@ -1,4 +1,4 @@
-include "ntt_rec2.dfy"
+include "ntt_rec3.dfy"
 include "index.dfy"
 
 module ntt {
@@ -14,6 +14,7 @@ module ntt {
     import opened rindex
 
     import opened ntt_recs2
+    import opened ntt_recs3
 
     lemma index_bounded_lemma(
         j: nat, k: nat, ki: nat,
@@ -46,172 +47,210 @@ module ntt {
         }
     }
 
-    // lemma ntt_chunk_base_case(a': seq<elem>, 
-    //     k: nat, ki: nat, t: elem, u: elem,
-    //     m: pow2_t)
+    type n_sized = s: seq<elem>
+        | |s| == N == pow2(L).full witness *
 
-    //     requires |a'| == N == pow2(L).full;
-    //     requires m.exp == 1;
-    //     requires ki < pow2_div(pow2(L), m).full;
-    //     requires k == ki * m.full;
-    //     requires k < k + 1 < N;
+    function method chunk_count(len: pow2_t): pow2_t
+        requires 0 <= len.exp <= L;
+    {
+        pow2_div(pow2(L), len)
+    }
 
-    //     requires t == modmul(1, Ar()[k + 1]);
-    //     requires u == Ar()[k];
-    //     requires a'[k] == modadd(u, t);
-    //     requires a'[k+1] == modsub(u, t);
+    lemma chunk_index_bounded(len: pow2_t, ki: nat)
+        requires 0 <= len.exp <= L;
+        requires ki < chunk_count(len).full;
+        ensures 0 <= ki * len.full <= N - len.full;
+    {
+        var max_count := pow2_div(pow2(L), len).full;
+        var csize := len.full;
+        nth_root_lemma();
+        calc {
+            ki * csize;
+        <=  { LemmaMulUpperBound(ki, max_count - 1, csize, csize); }
+            (max_count - 1) * csize;
+            { LemmaMulIsCommutativeAuto(); }
+            csize * (max_count - 1);
+            { LemmaMulIsDistributiveSubAuto(); }
+            max_count * csize - 1 * csize;
+            N -  csize;
+        }
+        LemmaMulNonnegative(ki, csize);
+    }
 
-    //     ensures Ar()[k..k+2] == get_level_chunk(m, ki);
-    //     ensures a'[k] == poly_eval(get_level_chunk(m, ki), omega_nk(m, 0));
-    //     ensures a'[k+1] == poly_eval(get_level_chunk(m, ki), omega_nk(m, 1));
+    lemma chunk_index_bounded_auto(len: pow2_t)
+        requires 0 <= len.exp <= L;
+        ensures forall ki | 0 <= ki < chunk_count(len).full ::
+            0 <= ki * len.full <= N - len.full;
+    {
+        forall ki |  0 <= ki < chunk_count(len).full 
+            ensures 0 <= ki * len.full <= N - len.full;
+        {
+            chunk_index_bounded(len, ki);
+        }
+    }
+
+    predicate n_sized_diff_chunk(y: n_sized, y': n_sized, len: pow2_t, ki: nat)
+        requires 0 <= len.exp <= L;
+        requires ki < chunk_count(len).full;
+    {
+        var offset := ki * len.full;
+        chunk_index_bounded(len, ki);
+        forall i | (0 <= i < offset || offset + len.full <= i < N) :: 
+            y'[i] == y[i] 
+    }
+
+    function view_as_chunks(y: n_sized, len: pow2_t): seq<seq<elem>>
+        requires 0 <= len.exp <= L;
+    {
+        var max_count := pow2_div(pow2(L), len).full;
+        var csize := len.full;
+        chunk_index_bounded_auto(len);
+        seq(max_count, ki requires 0 <= ki < max_count => y[ki * csize..ki * csize + csize])
+    }
+
+    function view_as_chunks_prefix(y: n_sized, len: pow2_t, i: nat): seq<seq<elem>>
+        requires 0 <= len.exp <= L;
+        requires i <= pow2_div(pow2(L), len).full;
+    {
+        var max_count := pow2_div(pow2(L), len).full;
+        var count := i;
+        var csize := len.full;
+        chunk_index_bounded_auto(len);
+        seq(count, ki requires 0 <= ki < count => y[ki * csize..ki * csize + csize])    
+    }
+
+    function view_as_chunks_suffix(y: n_sized, len: pow2_t, i: nat): seq<seq<elem>>
+        requires 0 <= len.exp <= L;
+        requires i <= pow2_div(pow2(L), len).full;
+    {
+        var max_count := pow2_div(pow2(L), len).full;
+        var count := max_count - i;
+        var csize := len.full;
+        chunk_index_bounded_auto(len);
+        seq(count, ki requires 0 <= ki < count => y[ki * csize..ki * csize + csize]) 
+    }
+
+    // lemma chunks_view_update(y: n_sized, y': n_sized,
+    //     len1: pow2_t, view1: seq<seq<elem>>,
+    //     len2: pow2_t, view2: seq<seq<elem>>,
+    //     ki: nat)
+    //     requires ki < |view2|;
+    //     requires 1 <= len2.exp <= L;
+    //     requires len1 == pow2_half(len2);
+    //     requires view_as_chunks(y, len1) == view1;
+    //     requires view_as_chunks(y, len2) == view2;
+    //     requires forall i | 0 <= i < ki * len2.full < N :: y'[i] == y[i];
+    //     requires forall i | 0 <= ki * len2.full <= i < N :: y'[i] == y[i];
     // {
-    //     pow2_basics(m);
-    //     var m' := pow2_half(m);
 
-    //     assert t == Ar()[k + 1] by {
-    //         assert Ar()[k + 1] < Q;
-    //     }
-
-    //     var even := Ar()[k..k+1];
-    //     var odd := Ar()[k+1..k+2];
-    //     var chunk :=Ar()[k..k+2];
-    //     assert chunk == even + odd;
-
-    //     var original := orignal_index(ki, 0, m);
-    //     assert original.v == k;
-
-    //     ntt_rec_base_case(odd, m');
-    //     ntt_rec_base_case(even, m');
-
-    //     assert u == poly_eval(even, omega_nk(m', 0));
-    //     assert t == poly_eval(odd, omega_nk(m', 0));
-
-    //     var omg := omega_nk(m, 0);
-
-    //     calc == {
-    //         modmul(omg, t);
-    //         {
-    //             LemmaPow0(omega_n(m));
-    //         }
-    //         modmul(1, t);
-    //     }
-
-    //     y_k_value(chunk, even, odd, pow2(0), pow2(1),
-    //         omg, 0, u, t, a'[k]);
-
-    //     y_k'_value(chunk, even, odd, pow2(0), pow2(1),
-    //         omg, 0, u, t, a'[k+1]);
-
-    //     // assert |get_level_chunk(m, ki)| == 2;
-    //     assume Ar()[k..k+2] == get_level_chunk(m, ki);
-    // }
-
-    // function view_as_chunks(y: seq<elem>, len: pow2_t): seq<seq<elem>>
-    //     requires |y| == N == pow2(L).full
-    //     requires 1 <= len.exp <= L
-    // {
-    //     var count := pow2_div(pow2(L), len).full;
-    //     var csize := len.full;
-    //     assert forall ki |  0 <= ki < count :: 0 <= ki * csize <= N - csize by {
-    //         forall ki |  0 <= ki < count 
-    //             ensures 0 <= ki * csize <= N - csize
-    //         {
-    //             nth_root_lemma();
-    //             calc {
-    //                 ki * csize;
-    //             <=  { LemmaMulUpperBound(ki, count - 1, csize, csize); }
-    //                 (count - 1) * csize;
-    //                 { LemmaMulIsCommutativeAuto(); }
-    //                 csize * (count - 1);
-    //                 { LemmaMulIsDistributiveSubAuto(); }
-    //                 count * csize - 1 * csize;
-    //                 N -  csize;
-    //             }
-    //             LemmaMulNonnegative(ki, csize);
-    //         }
-    //     }
-    //     seq(count, ki requires 0 <= ki < count => y[ki * csize..ki * csize + csize])
     // }
 
     // predicate ntt_chunk_loop_inv(
     //     y: seq<elem>,
-    //     m: pow2_t,
-    //     ki: nat,
+    //     m: pow2_t, 
     //     a: seq<seq<elem>>,
-    //     idxs: seq<seq<index_t>>)
+    //     idxs: seq<seq<index_t>>,
+    //     ki: nat)
+    //     requires |y| == N == pow2(L).full
+    //     requires 1 <= m.full;
+    //     requires 0 <= m.exp <= L;
+    //     requires ki < pow2_div(pow2(L), m).full;
     //     requires ntt_chunk_indicies_inv(a, idxs, m);
     // {
-    //     view_as_chunks(y, m)[ki] == ntt_rec2(a[ki], m, idxs[ki], ki)
+    //     view_as_chunks(y, m)[..ki] == ntt_rec3(a, m, idxs)[..ki]
     // }
 
-    method ntt_chunk_loop(
-        y: seq<elem>,
-        k: nat,
-        m: pow2_t,
-        ghost ki: nat,
-        ghost a: seq<seq<elem>>,
-        ghost idxs: seq<seq<index_t>>)
+    // lemma init_implies_inv(
+    //     y: seq<elem>,
+    //     m: pow2_t, 
+    //     a: seq<seq<elem>>,
+    //     idxs: seq<seq<index_t>>)
 
-    returns (y': seq<elem>)
-        requires ntt_chunk_indicies_inv(a, idxs, m);
-        // this loop works on a chunk of size m.full
-        // by combining two smaller chunks of size m.full/2
-        // m.full: the chunk size at the current level
-        requires |y| == N == pow2(L).full;
-        // m.exp: the level, go from 1 to L (log N)
-        // ki: the chunk id at current level, go from 0 to N/m
-        requires ki < pow2_div(pow2(L), m).full;
-        // k is ki times chunk size, points to start of the chunk
-        requires k == ki * m.full;
-        requires m.exp == 1 ==> y == Ar();
-    {
-        y' := y;
-        var len' := pow2_half(m);
-        var omgm := omega_n(m);
+    //     requires |y| == N == pow2(L).full
+    //     requires 1 == m.full;
+    //     requires 0 == m.exp;
+    //     requires ntt_chunk_indicies_inv(a, idxs, m);
+    //     requires y == Ar();
+    //     ensures ntt_chunk_loop_inv(y, m, a, idxs);
+    // {
+    //     var view := view_as_chunks(y, m);
+    //     var base := ntt_rec3_base(a, m, idxs);
+    //     forall ki | 0 <= ki < N
+    //         ensures view[ki] == base[ki];
+    //     {
+    //         calc == {
+    //             view[ki];
+    //             y[ki..ki+1];
+    //             [y[ki]];
+    //             [Ar()[ki]];
+    //             base[ki];
+    //         }
+    //     }
+    // }
 
-        var omg := 1;
-        var j := 0;
+    // method ntt_chunk_loop(
+    //     y: seq<elem>,
+    //     k: nat,
+    //     m: pow2_t,
+    //     ghost ki: nat,
+    //     ghost a: seq<seq<elem>>,
+    //     ghost idxs: seq<seq<index_t>>)
 
-        assert omg == modpow(omgm, 0) by {
-            LemmaPow0Auto();
-        }
+    // returns (y': seq<elem>)
+    //     requires 1 <= m.exp <= L;
+    //     requires ntt_chunk_indicies_inv(a, idxs, pow2_half(m));
+    //     requires |y| == N == pow2(L).full;
+    //     requires ki < pow2_div(pow2(L), m).full;
+    //     requires k == ki * m.full;
+    //     requires ntt_chunk_loop_inv(y, pow2_half(m), a, idxs, ki);
+    // {
+    //     y' := y;
+    //     var len' := pow2_half(m);
+    //     var omgm := omega_n(m);
 
-        pow2_basics(m);
+    //     var omg := 1;
+    //     var j := 0;
 
-        index_bounded_lemma(0, k, ki, m);
+    //     assert omg == modpow(omgm, 0) by {
+    //         LemmaPow0Auto();
+    //     }
 
-        // ghost var y_o := y[k..k+len'.full];
-        // ghost var y_e := y[k+len'.full..k+m.full];
-        // ghost var y_ks := compute_y_ks(a[ki], y_e, y_o, m);
+    //     pow2_basics(m);
 
-        while (j < len'.full)
-            invariant 0 <= j <= len'.full;
-            invariant omg == modpow(omgm, j);
-            invariant |y'| == |y|;
-            invariant k + j + len'.full <= N;
-            invariant y[..k] == y'[..k];
-            invariant y[k+j..k+len'.full] == y'[k+j..k+len'.full];
-            invariant y[k+len'.full+j..] == y'[k+len'.full+j..];
-        {
-            index_bounded_lemma(j, k, ki, m);
-            var t := modmul(omg, y[k + j + len'.full]);
-            var u := y[k + j];
-            y' := y'[k + j := modadd(u, t)];
-            y' := y'[k + j + len'.full := modsub(u, t)];
+    //     index_bounded_lemma(0, k, ki, m);
 
-            omg_inv(omgm, omg, m, j);
-            omg := modmul(omg, omgm);
-            j := j + 1;
+    //     // ghost var y_o := y[k..k+len'.full];
+    //     // ghost var y_e := y[k+len'.full..k+m.full];
+    //     // ghost var y_ks := compute_y_ks(a[ki], y_e, y_o, m);
 
-            // if m.exp == 1 {
-            //    ghost var y_exp := ntt_rec2_base(a[ki], m, idxs[ki], ki);
-            //    assert y'[k..k+2] == y_exp; 
-            // }
-        }
+    //     while (j < len'.full)
+    //         invariant 0 <= j <= len'.full;
+    //         invariant omg == modpow(omgm, j);
+    //         invariant |y'| == |y|;
+    //         invariant k + j + len'.full <= N;
+    //         invariant y[..k] == y'[..k];
+    //         invariant y[k+j..k+len'.full] == y'[k+j..k+len'.full];
+    //         invariant y[k+len'.full+j..] == y'[k+len'.full+j..];
+    //     {
+    //         index_bounded_lemma(j, k, ki, m);
+    //         var t := modmul(omg, y[k + j + len'.full]);
+    //         var u := y[k + j];
+    //         y' := y'[k + j := modadd(u, t)];
+    //         y' := y'[k + j + len'.full := modsub(u, t)];
 
-        // assert y[..k] == y'[..k];
-        // assert y[k+m.full..] == y'[k+m.full..];
-    }
+    //         omg_inv(omgm, omg, m, j);
+    //         omg := modmul(omg, omgm);
+    //         j := j + 1;
+
+    //         // if m.exp == 1 {
+    //         //    ghost var y_exp := ntt_rec2_base(a[ki], m, idxs[ki], ki);
+    //         //    assert y'[k..k+2] == y_exp; 
+    //         // }
+    //     }
+
+    //     // assert y[..k] == y'[..k];
+    //     // assert y[k+m.full..] == y'[k+m.full..];
+    // }
 
     // method ntt_level_loop(a: seq<elem>, s: nat)
     //     requires |a| == N == pow2(L).full;
